FunctionAppLemmas.v
@@ -4,12 +4,12 @@ Local Open Scope type_scope.
 
 (** We apply AC_∞, the type-theoretic axiom of choice, so that
           we don't need to do higher order unification later. *)
-Lemma emptiesStackStep' message input world pf
+Lemma emptiesStackStep' input world pf
       (H : forall i : input,
-             { p' : stackProcess message input world
-             & emptiesStack (stackTransition (inr i) pf) p' *
+             { p' : stackProcess input world
+             & emptiesStack (stackTransition i pf) p' *
                emptiesStackForever p' })
-: @emptiesStackForever message input world (Step pf).
+: @emptiesStackForever input world (Step pf).
 Proof.
   econstructor.
   intro i.
@@ -17,7 +17,7 @@ Proof.
   split; apply (projT2 (H _)).
 Defined.
 
-Definition stackProcess_eta message input world (p : stackProcess message input world)
+Definition stackProcess_eta input world (p : stackProcess input world)
 : p = match p with
         | Step f => Step f
       end.
@@ -33,15 +33,15 @@ Proof.
   destruct p; reflexivity.
 Defined.
 
-Lemma emptiesStackDone' message input world p q (H : p = q) : @emptiesStack message input world (stackDone, p) q.
+Lemma emptiesStackDone' input world p q (H : p = q) : @emptiesStack input world (stackDone, p) q.
 Proof.
   subst.
   constructor.
 Defined.
 
-Lemma emptiesStackPush_sigT {message input world} (m : message) (sw : stackWorld message world)
+Lemma emptiesStackPush_sigT {input world} (m : input) (sw : stackWorld input world)
       (pf : stackStep) P
-: { p2 : stackProcess message input world & emptiesStack (stackTransition (inl m) pf) p2 * { p3 : _ & emptiesStack (sw, p2) p3 * P p3 } }
+: { p2 : stackProcess input world & emptiesStack (stackTransition m pf) p2 * { p3 : _ & emptiesStack (sw, p2) p3 * P p3 } }
   -> { p3 : _ & emptiesStack (stackPush m sw, Step pf) p3 * P p3 }.
 Proof.
   intro H.
@@ -52,8 +52,8 @@ Proof.
         | apply (snd (projT2 (snd (projT2 H)))) ].
 Defined.
 
-Lemma emptiesStackLift_sigT {message input world} (a : action world) (sw : stackWorld message world)
-      (p : stackProcess message input world) P
+Lemma emptiesStackLift_sigT {input world} (a : action world) (sw : stackWorld input world)
+      (p : stackProcess input world) P
 : { p2 : _ & emptiesStack (sw, p) p2 * P p2 }
   -> { p2 : _ & emptiesStack (stackLift a sw, p) p2 * P p2 }.
 Proof.
@@ -64,7 +64,7 @@ Proof.
         | apply (snd (projT2 H)) ].
 Defined.
 
-Lemma emptiesStackDone_sigT {message input world} p (P : stackProcess message input world -> Type)
+Lemma emptiesStackDone_sigT {input world} p (P : stackProcess input world -> Type)
 : P p -> { p' : _ & emptiesStack (stackDone, p) p' * P p' }.
 Proof.
   intro H.
@@ -72,10 +72,10 @@ Proof.
   split; [ eapply emptiesStackDone | ]; eassumption.
 Defined.
 
-Lemma emptiesStackPush_ex {message input world} (m : message) (sw : stackWorld message world)
+Lemma emptiesStackPush_ex {input world} (m : input) (sw : stackWorld input world)
       (pf : stackStep) P
-: (exists p2 : stackProcess message input world,
-     emptiesStack (stackTransition (inl m) pf) p2
+: (exists p2 : stackProcess input world,
+     emptiesStack (stackTransition m pf) p2
      /\ exists p3 : _, emptiesStack (sw, p2) p3 /\ P p3)
   -> exists p3 : _, emptiesStack (stackPush m sw, Step pf) p3 /\ P p3.
 Proof.
@@ -85,8 +85,8 @@ Proof.
   eassumption.
 Defined.
 
-Lemma emptiesStackLift_ex {message input world} (a : action world) (sw : stackWorld message world)
-      (p : stackProcess message input world) P
+Lemma emptiesStackLift_ex {input world} (a : action world) (sw : stackWorld input world)
+      (p : stackProcess input world) P
 : (exists p2 : _, emptiesStack (sw, p) p2 /\ P p2)
   -> exists p2 : _, emptiesStack (stackLift a sw, p) p2 /\ P p2.
 Proof.
@@ -96,7 +96,7 @@ Proof.
   eassumption.
 Defined.
 
-Lemma emptiesStackDone_ex {message input world} p (P : stackProcess message input world -> Prop)
+Lemma emptiesStackDone_ex {input world} p (P : stackProcess input world -> Prop)
 : P p -> exists p' : _, emptiesStack (stackDone, p) p' /\ P p'.
 Proof.
   intro H.
